clean and document factor_matrix

mathematica_examples/factor_matrix.lean
@@ -4,9 +4,12 @@ Released under Apache 2.0 license as described in the file LICENSE.
 Author: Robert Y. Lewis
 -/
 
-import init.meta.mathematica .bquant .datatypes
-open expr tactic
+import init.meta.mathematica .bquant .datatypes .and_of_map ..data.rat .comp_val
+open expr tactic rat
 
+/-
+For this example, we give a very brief development of matrices as lists of lists.
+-/
 
 @[reducible]
 def {u} ith {α : Type u} [inhabited α] (l : list α) (i : ℕ) : α :=
@@ -15,14 +18,23 @@ match l^.nth i with
 | none   := default α
 end
 
+/--
+The transpose of a list-of-lists matrix
+-/
 def {u} transpose_list {α : Type u} [inhabited α] (m : list (list α)) : list (list α) :=
 list.map (λ i, m^.map (λ l, ith l i)) (native.upto (ith m 0)^.length)
 
+/--
+The dot product of two list "vectors"
+-/
 def {u} dot_lists {α : Type u} [has_zero α] [has_mul α] [has_add α] : list α → list α → α
 | [a] [b] := a*b
 | (h1::t1) (h2::t2) := h1*h2 + dot_lists t1 t2
 | _ _ := 0
 
+/--
+The product of two list-of-lists matrices
+-/
 def {u} mul_lists {α : Type u} [has_zero α] [has_mul α] [has_add α] [inhabited α]
        (m1 m2 : list (list α))  : list (list α) :=
 list.map (λ i, (list.map (λ j, dot_lists (ith m1 i) (ith (transpose_list m2) j)) 
@@ -32,16 +44,119 @@ infix `**`:50 := mul_lists
 
 @[reducible]
 def {u} is_lower_triangular {α : Type u} [has_lt α] [has_zero α] (m : list (list α)) : Prop :=
-∀ i < m^.length, ∀ j < (ith m i)^.length, i < j → ith (ith m i) j = 0
+∀ i : fin (m^.length), ∀ j : fin ((ith m i^.val)^.length), i^.val < j^.val → ith (ith m i^.val) j^.val = 0
 
 @[reducible]
 def {u} is_upper_triangular {α : Type u} [has_lt α] [has_zero α] (m : list (list α)) : Prop :=
-∀ i < m^.length, ∀ j < (ith m i)^.length, i > j → ith (ith m i) j = 0
+∀ i : fin (m^.length), ∀ j : fin ((ith m i^.val)^.length), i^.val > j^.val → ith (ith m i^.val) j^.val = 0
 
+
+
+
+
+/-
+On data types with decidable (in)equality, we can simplify the implementation using this tactic
+to do arithmetic. However, it can be slow.
+-/
 meta def dec_triv_tac : tactic unit :=
 do t ← target,
    to_expr `(dec_trivial : %%t) >>= apply
 
+/--
+Takes an expression of the form a < b, tries to find a proof that a ≥ b, and applies absurd.
+-/
+meta def dec_false (e : expr) : tactic unit :=
+do md ← mk_mvar, md2 ← mk_mvar,
+   tp ← infer_type e,
+   (do to_expr `(%%md < %%md2) >>= unify tp,
+   nmd ← ((do (v,_) ← instantiate_mvars md >>= norm_num,return v) <|> (make_expr_into_num md)), 
+   nmd2 ← ((do (v,_) ← instantiate_mvars md2 >>= norm_num, return v) <|> (make_expr_into_num md2)), 
+   ge ← to_expr `(%%nmd ≥ %%nmd2),
+   gep ← mk_inhabitant_using ge gen_comp_val,
+   to_expr `(absurd %%e (not_lt_of_ge %%gep)) >>= apply)
+
+meta def unify_with_eq (e : expr) : tactic (expr × expr) :=
+do e1 ← mk_mvar, e2 ← mk_mvar,
+   to_expr `(%%e1 = %%e2) >>= unify e,
+   return $ (e1, e2)
+
+meta def triangularity_tac_aux : tactic unit :=
+do t ← target, i ← mk_mvar, j ← mk_mvar, P ← mk_mvar, 
+target >>= whnf >>= change,  
+dsimp,
+to_expr `(%%i < %%j → %%P) >>= unify t, 
+ h ← mk_fresh_name >>= intro, 
+(dec_false h  <|> do 
+ (e1, e2) ← target >>= unify_with_eq, to_expr `(%%e1 = %%e2) >>= change, 
+ reflexivity)
+
+/--
+Tries to automatically solve goals of the form is_(upper/lower)_triangluar m,
+by transforming the quantifications to conjunctions and testing for 0s.
+-/
+meta def triangularity_tac : tactic unit := solve1 $
+do dsimp, aom ← mk_mvar,
+   refine `(forall_of_and_of_map %%aom),
+   repeat (applyc `and.intro),
+   all_goals $ solve1 $ 
+     (do aom' ← mk_mvar, 
+         refine `(forall_of_and_of_map %%aom'), 
+         repeat (applyc `and.intro), 
+         all_goals (triangularity_tac_aux))
+
+
+meta def refine_lhs : expr → expr → (expr → expr → tactic expr) → tactic expr
+| lhs ```(list.cons %%h %%t) f :=
+  do v1 ← mk_mvar, v2 ← mk_mvar,
+     to_expr `(%%v1 :: %%v2) >>= unify lhs,
+     rc ← refine_lhs v2 t f,
+     nh ← f v1 h,
+     to_expr `(%%nh::%%rc)
+| lhs ```(@list.nil %%t) _ := to_expr `(@list.nil %%t)
+| _ _ _ := failed
+
+/--
+When rhs is a list of lists, refine_lhs_outer lhs rhs tries to unify
+lhs to the same form as rhs. E.g., if rhs is [[1, 2], [3, 4]], will try to
+match lhs to [[a, b], [c, d]].
+-/
+meta def refine_lhs_outer (lhs rhs : expr) : tactic expr :=
+refine_lhs lhs rhs (λ e1 e2, refine_lhs e1 e2 (λ e3 e4, return e3))
+
+/--
+Proves that the product of two list-of-lists matrices is another list-of-lists matrix.
+-/
+meta def mk_mul_prf : tactic unit :=
+do t ← target,
+   lhs ← mk_mvar, rhs ← mk_mvar,
+   to_expr `(%%lhs = %%rhs) >>= unify t,
+   e ← whnf rhs >>= refine_lhs_outer lhs,
+   to_expr `(%%e = %%rhs) >>= change,
+   repeat 
+     (do applyc `congr_helper,
+     repeat 
+       (do applyc `congr_helper,
+       dsimp,
+       t ← target,
+       [_, lhs, rhs] ← return $ get_app_args t,
+       lhs' ← make_expr_into_sum lhs,
+       to_expr `(%%lhs' = %%rhs) >>= change,
+       (_, prf) ← norm_num lhs',
+       apply prf), 
+     reflexivity),
+   cleanup, reflexivity
+
+/-
+lu_tac looks for a target of the form 
+∃ l u, is_lower_triangluar l ∧ is_upper_triangular u ∧ l**u = M
+where M is a matrix, and proves this using Mathematica's LUDecomposition.
+matrix_factor.m is an extra file that defines LUDecomp, a variant on LUDecomposition
+that returns more appropriate data.
+
+In general, the product l**u is only equal to M up to a row permutation.
+This tactic does not handle that; it will only succeed if the permutation is the identity.
+We leave it as an exercise for the reader to extend!
+-/
 meta def lu_tac : tactic unit := 
 do t ← target, 
    (lam _ _ _ bd) ← return $ app_arg t,
@@ -55,12 +170,20 @@ do t ← target,
    m2 ← to_expr `((%%m : list %%tp)),
    lhs ← to_expr `(ith %%m2 0), rhs ← to_expr `(ith %%m2 1),
    existsi lhs, existsi rhs,
-   split, dec_triv_tac, split, dec_triv_tac, reflexivity
+   split, triangularity_tac, split, triangularity_tac, mk_mul_prf
 
 
-example : ∃ l u, is_lower_triangular l ∧ is_upper_triangular u ∧ mul_lists l u = [[(1 : ℤ), 2], [3, 4]] := 
+-- the examples below take a few seconds to run, and can bog down the editor.
+-- remove the #exit command to try them.
+#exit
+
+example : ∃ l u, is_lower_triangular l ∧ is_upper_triangular u ∧ l ** u = [[(1 : ℤ), 2], [3, 4]] := 
 by lu_tac
 
 example : ∃ l u, is_lower_triangular l ∧ is_upper_triangular u
-             ∧ l ** u = [[1, 2, 3], [1, 4, 9], [1, 8, 27]] := 
+             ∧ l ** u = [[(1 : ℤ), 2, 3], [1, 4, 9], [1, 8, 27]] := 
+by lu_tac
+
+example : ∃ l u, is_lower_triangular l ∧ is_upper_triangular u
+             ∧ l ** u = [[(1 : ℝ), 2, 3, 4, 5],  [0, -1, 3, -5, 8], [1, 4, 9, 10, 20], [1, -1, 0, -10, 5], [1, 8, 27, -11, 0]] := 
 by lu_tac
